\documentclass[11pt]{article}

% --- Encoding & Language ---
\usepackage[utf8]{inputenc}
\usepackage[T1]{fontenc}
\usepackage[english]{babel}

% --- Math Packages ---
\usepackage{amsmath, amssymb, amsfonts}
\usepackage{mathtools}
\usepackage{physics}          % for \dv, \pdv, \grad, etc.
\usepackage{bm}               % for bold math symbols
\usepackage{siunitx}          % for units

% --- Page Layout ---
\usepackage[margin=1in]{geometry}
\usepackage{setspace}
\onehalfspacing

% --- Theorem Environment ---
\usepackage{amsthm}
% Create a shared counter (let's call it 'statement') per section
\newtheorem{statement}{Statement}[section]
\newtheorem{theorem}[statement]{Theorem}
 
% Define 'assumption' and 'diagram' to use the same counter
\newtheorem{assumption}[statement]{Assumption}
\newtheorem{diagram}[statement]{Diagram}
\newtheorem{note}[statement]{Note}

% --- Figure & Table ---
\usepackage{graphicx}
\usepackage{float}
\usepackage{caption}
\usepackage{subcaption}
\usepackage{mwe}
% \includegraphics{example-image}
\usepackage{hyperref}

% --- TikZ for Diagrams ---
\usepackage{tikz}
\usetikzlibrary{arrows.meta, decorations.pathmorphing, patterns}

% --- Code Listings (optional) ---
\usepackage{listings}
\lstset{
  basicstyle=\ttfamily\small,
  frame=single,
  breaklines=true,
  postbreak=\mbox{\textcolor{red}{$\hookrightarrow$}\space},
}


% --- Title Info ---
\title{\textbf{Force Based Model Analysis}}
\author{Jerry Wu}
\date{\today}

\begin{document}

\maketitle
\noindent
\textbf{Helpful Link:}
\begin{itemize}
    \item \href{https://www.geogebra.org/classic/vzgc97bq}{Geogebra Demo}
    \item \href{https://www.canva.com/design/DAGo-OCr6Yo/K5YV57vaBxux-PqkqwI4ow/edit?utm_content=DAGo-OCr6Yo&utm_campaign=designshare&utm_medium=link2&utm_source=sharebutton}{Canva Graphics}
\end{itemize}

\begin{assumption}\label{ass:leg-ground-contact}
The end point of each leg is always contacting the ground.=
\end{assumption}

\begin{assumption}\label{ass: no-body-contact}
The robot body would never contact with the terrain
\end{assumption}

\section{Statics}
\begin{assumption}
Static means the robot would not move and achieve static equilibrium in this state
\end{assumption}
\subsection*{Slope}

\begin{diagram}
    Simple case where two legs have same height
\end{diagram}\label{ass:h2-equal-h1}
\vspace{1ex} % small vertical space
\begin{center}
    \includegraphics[width=0.6\textwidth]{figs/Simple case where two legs have same height.jpg} % replace with your image
\end{center}

To start with,  we put robot on a slope with angle \(\theta\). To make the analysis easier,
assume that two leg have same height \(h\) in this case. Therefore, the moment arm are symetric
for \(R_A\) and \(R_B\). Therefore, we can get follow equations:
\[ \sum F_x = (f_1+f_2) - \sin(\theta)mg = 0 \]
\[ \sum F_y = (N_A+N_B) - \cos(\theta)mg = 0 \]
\[ \sum M_A = L_\text{spine} \cdot N_B -  L \cdot mg \cdot \sin(\frac{\pi}{2}-\phi+\theta) = 0 \]
\[ \sum M_B = L_\text{spine} \cdot N_A -  L \cdot mg \cdot \sin(\frac{\pi}{2}-\phi+\theta) = 0 \]

\begin{diagram}
    Two legs have different height
\end{diagram}\label{ass:h2-larger-than-h1}
\vspace{1ex} % small vertical space
\begin{center}
    \includegraphics[width=0.5\textwidth]{figs/Two legs have different height.jpg} % replace with your image
\end{center}

Now extend the case to where the leg length would change. Here the robot extended
the right leg to \(h_2\), which makes the robot rotate angle \(\beta\) around
the z-Axis. Now both moment arms on two legs are 
shifted. We can also form the static equilibrium equation as follows:

\[ \sum F_x = (f_1+f_2) - \sin(\theta)mg = 0 \]
\[ \sum F_y = (N_A+N_B) - \cos(\theta)mg = 0 \]
\[ \sum M_A = \frac{L_\text{spine}}{\sin(\frac{\pi}{2}-\beta)} \cdot N_B \cdot \sin(\frac{\pi}{2})-  L_1 \cdot mg \cdot \sin(\frac{\pi}{2}-\phi_1+\theta) = 0 \]
\[ \sum M_B = \frac{L_\text{spine}}{\sin(\frac{\pi}{2}-\beta)} \cdot N_A \cdot \sin(\frac{\pi}{2})-  L_2 \cdot mg \cdot \sin(\frac{\pi}{2}-\phi_2-\theta) = 0 \]

based on the geometry of our robot, we can also formulate:
\[L_\text{spine} \cdot \cos(\frac{\pi}{2}-\beta) = h_2 - h_1 \]

\begin{note}\label{not:what-is-known}
\(h_1\), \(h_2\) are known values, so \(\beta\) is also known.  
Therefore, \(\phi_1\) and \(\phi_2\) can easily be solved using Theorem~\ref{thm:law-of-cosines}.
\end{note}

\begin{theorem}\label{thm:law-of-cosines}
Law of Cosines

\[
\cos A = \frac{b^2 + c^2 - a^2}{2bc}
\]
\[
\cos B = \frac{a^2 + c^2 - b^2}{2ac}
\]
\[
\cos C = \frac{a^2 + b^2 - c^2}{2ab}
\]
\end{theorem}


\subsection*{Zig-Zag Terrain}

\begin{assumption}\label{ass:Zig-Zag-terrain-assumption}
The terrain is uniform that all triangle obstable and gap between them are same
\end{assumption}

A natural extension for the slope is triangle terrain. There are esseintially five cases
when robot is static on the triangle terrain: 1. two legs on the same slope 2. two legs on two slopes that face each other
3. two legs on two slopes that does not face each other 4. one leg is on the slope and the other is on the gap. 5. two legs
are all on the gap. 

For case 1, we have already discussed in the previous section. And for case 5, it is esseintially the same
like slope when \(\theta\) is 0.

\begin{diagram}
    Case2: two legs on the slope that face each other
\end{diagram}
\vspace{1ex} % small vertical space
\begin{center}
    \includegraphics[width=0.7\textwidth]{figs/Case2.jpg} % replace with your image
\end{center}

To make it clearer, I changed the coordinate that aligns with the ground rather slope from now on.
We can also formulate the equilibrium equations:

\[ \sum F_x = (-f_1+f_2)\cos(\theta) + (N_A-N_B) \sin(\theta) = 0 \]
\[ \sum F_y = (f_1+f_2)\sin(\theta) + (N_A+N_B) \cos(\theta) - mg = 0 \]
\[ \sum M_A =  L_\text{Arm} \cdot (N_B \cdot \sin(\frac{\pi}{2}-\omega_2) + f_2 \cdot \sin(\pi-\omega_2)) - L_1\cdot mg \cdot \sin(\mu_1)= 0 \]
\[ \sum M_B =  L_\text{Arm} \cdot (N_B \cdot \sin(\frac{\pi}{2}-\omega_1) + f_1 \cdot \sin(\pi-\omega_1)) - L_2\cdot mg \cdot \sin(\mu_2)= 0 \]

where by geometry of the shape, we can find:
\[\omega_1 = (\theta + \beta)  - (\frac{\pi}{2}-\alpha) \]
\[\omega_2 = (\theta - \beta) + (\frac{\pi}{2}-\alpha) \]
\[\mu_1 = \pi-(\phi_1+\omega_1)-(\frac{\pi}{2}-\theta) \]
\[\mu_2 = \pi-(\phi_2+\omega_2)-(\frac{\pi}{2}-\theta) \]
\[\alpha = \arctan(\frac{L_\text{Spine}}{h2-h1}) \]
\[L_\text{Arm} = \sin(\alpha) \cdot L_\text{Spine}\]

similarly to Note~\ref{not:what-is-known}, this equalion can be solved.

\begin{diagram}
    Case3: two legs on two slopes that do not face each other
\end{diagram}
\vspace{1ex} % small vertical space
\begin{center}
    \includegraphics[width=0.7\textwidth]{figs/Case3.jpg} % replace with your image
\end{center}

\[ \sum F_x = (f_1-f_2)\cos(\theta) + (-N_A+N_B) \sin(\theta) = 0 \]
\[ \sum F_y = (f_1-f_2)\sin(\theta) + (-N_A+N_B) \cos(\theta) - mg = 0 \]
\[ \sum M_A =  L_\text{Arm} \cdot (N_B \cdot \sin(\pi-\omega_2) + f_2 \cdot \sin(\frac{\pi}{2}-\omega_2)) - L_1\cdot mg \cdot \sin(\mu_1)= 0 \]
\[ \sum M_B =  L_\text{Arm} \cdot (N_A \cdot \sin(\pi-\omega_1) + f_1 \cdot \sin(\frac{\pi}{2}-\omega_1)) - L_2\cdot mg \cdot \sin(\mu_2)= 0 \]

where by geometry of the shape, we can find:
\[\omega_1 = \beta + \alpha - \theta\]
\[\omega_2 =  \pi - \beta - \alpha - \theta\]
\[\mu_1 = \pi-(\phi_1+\omega_1)-\theta \]
\[\mu_2 = \pi-(\phi_2+\omega_2)-\theta \]
\[\alpha = \arctan(\frac{L_\text{Spine}}{h2-h1}) \]
\[L_\text{Arm} = \sin(\alpha) \cdot L_\text{Spine}\]

\begin{note}
The equation for \(\omega_1\)  can be found specifically by following equation:
\end{note}
\begin{equation}
x_1 + \phi_1 + \omega_1 + \theta = \pi
\end{equation}

\begin{equation}
\beta + x_1 + \phi_1 - \left( \frac{\pi}{2} - \alpha \right) = \frac{\pi}{2}
\end{equation}

\begin{equation}
\omega_1 = \beta + \alpha - \theta
\tag*{From (1) and (2)}
\end{equation}

\begin{diagram}
    Case4: one leg is on the slope and the other is on the gap
\end{diagram}
\vspace{1ex} % small vertical space
\begin{center}
    \includegraphics[width=0.7\textwidth]{figs/Case4.jpg} % replace with your image
\end{center}

\[ \sum F_x = -f_1 \cos(\theta) -f_2 + N_A \sin(\theta)= 0 \]
\[ \sum F_y = f_1 \sin(\theta)+ N_A \cos(\theta) + N_B - mg = 0 \]
\[ \sum M_A =  L_\text{Arm} \cdot (N_B \cdot \sin(\pi-\omega_2) + f_2 \cdot \sin(\frac{\pi}{2}-\omega_2)) - L_1\cdot mg \cdot \sin(\mu_1)= 0 \]
\[ \sum M_B =  L_\text{Arm} \cdot (N_B \cdot \sin(\pi-\omega_1) + f_1 \cdot \sin(\frac{3\pi}{2}-\omega_1)) - L_2\cdot mg \cdot \sin(\mu_2)= 0 \]

where by geometry of the shape, we can find:
\[\omega_1 = \theta - \beta + \alpha\]
\[\omega_2 =  \pi + \beta - \alpha \]
\[\mu_1 = \pi-(\phi_1+\omega_1)-\theta \]
\[\mu_2 = \pi-(\phi_2+\omega_2) \]
\[\alpha = \arctan(\frac{L_\text{Spine}}{h2-h1}) \]
\[L_\text{Arm} = \sin(\alpha) \cdot L_\text{Spine}\]

\begin{note}
The equation for \(\omega_1\)  can be found specifically by following equation:
\end{note}
\begin{equation}
x_1 + \phi_1 + \omega_1 = \pi
\end{equation}

\begin{equation}
\theta-\beta + x_1 + \phi_1 - \left( \frac{\pi}{2} - \alpha \right) = \frac{\pi}{2}
\end{equation}

\begin{equation}
\omega_1 = \theta - \beta + \alpha
\tag*{From (1) and (2)}
\end{equation}

Now, by observation, this case is very similar to previous case. In fact, all of the above cases
are geometrically similar, which means we can find a general expression for this force based model.

\begin{diagram}
    Determine the geometry shape by robot body and terrain
\end{diagram}
\vspace{1ex} % small vertical space
\begin{center}
    \includegraphics[width=0.5\textwidth]{figs/geometry shape.jpg} % replace with your image
\end{center}

After simplifying the model, it can be seen that given the terrain tangent angle \(\theta_1\), \(\theta_2\), robot pitch
angle \(\beta\) and length of the virtual link between end point of two leg \(L_{Arm}\) we can determine the triangle with
inner angle \(a,b,c\). 

Here is how we determine angle \(a, b, c\):
\[a = \pi - \theta_1 - \theta_2\]
\[b = \pi - \beta - \frac{\pi}{2}-(\frac{\pi}{2}-\alpha_L)-(\pi-\theta_1)\]
\[c = \pi - (\pi-\theta_2) + \beta - \alpha_L\]

by verification: 
\[a+b+c = \pi\]

As for different tangent angles, this property should hold as well. This means there would be \textbf{only one solution} by
given condition.

\begin{diagram}
    Generailized Free Body Diagram
\end{diagram}
\vspace{1ex} % small vertical space
\begin{center}
    \includegraphics[width=0.8\textwidth]{figs/Generailized.jpg} % replace with your image
\end{center}

Given the determined geometric shape of the robot and terrain, we can easily find the position of the COM through
the given of relative position \(L_1\) and \(L_2\), which can be solved by the geometry as well. Which means, if we put
the robot into coordinate, the points \((X_A, Y_A), (X_B, Y_B), (X_{COM}, Y_{COM})\) are given.


Therefore, given \((X_A, Y_A), (X_B, Y_B), (X_{COM}, Y_{COM}), \theta_1, \theta_2\), \(L_{Spine}\) we can formulate
\[
\sum \vec{F} = \vec{f}_1 + \vec{f}_2 + \vec{N}_A + \vec{N}_B + \vec{W} = \vec{0}
\]

\[
\sum \vec{M}_A = 
(\vec{r}_B - \vec{r}_A) \times (\vec{f}_2 + \vec{N}_B)
+ (\vec{r}_{\text{COM}} - \vec{r}_A) \times \vec{W}
= 0
\]

\[
\sum \vec{M}_B = 
(\vec{r}_A - \vec{r}_B) \times (\vec{f}_1 + \vec{N}_A)
+ (\vec{r}_{\text{COM}} - \vec{r}_B) \times \vec{W}
= 0
\]

where
\begin{align*}
\hat{t}_1 &= (\cos(\pi-\theta_1),\; \sin(\pi-\theta_1)) \quad \text{(contact tangent 1)} \\
\hat{n}_1 &= (-\sin(\pi-\theta_1),\; \cos(\pi-\theta_1)) \quad \text{(contact normal 1)} \\
\hat{t}_2 &= (\cos\theta_2,\; \sin\theta_2) \\
\hat{n}_2 &= (-\sin\theta_2,\; \cos\theta_2)
\end{align*}

\begin{align*}
\vec{f}_1 &= f_1 \cdot \hat{t}_1 = f_1 \cdot (\cos(\pi-\theta_1),\; \sin(\pi-\theta_1)) \\
\vec{N}_A &= N_A \cdot \hat{n}_1 = N_A \cdot (-\sin(\pi-\theta_1),\; \cos(\pi-\theta_1)) \\
\vec{f}_2 &= f_2 \cdot \hat{t}_2 = f_2 \cdot (\cos\theta_2,\; \sin\theta_2) \\
\vec{N}_B &= N_B \cdot \hat{n}_2 = N_B \cdot (-\sin\theta_2,\; \cos\theta_2) \\
\vec{W}   &= -mg \cdot (0,\; 1)
\end{align*}


\begin{align*}
\text{Moment arm of } \vec{f}_2, \vec{N}_B \text{ about A}: \quad
& \vec{r}_{f_2/A} = \vec{r}_B - \vec{r}_A = (X_B - X_A,\; Y_B - Y_A) \\
\text{Moment arm of } \vec{W} \text{ about A}: \quad
& \vec{r}_{W/A} = \vec{r}_{\text{COM}} - \vec{r}_A = (X_{COM} - X_A,\; Y_{COM} - Y_A) \\[1ex]
\text{Moment arm of } \vec{f}_1, \vec{N}_A \text{ about B}: \quad
& \vec{r}_{f_1/B} = \vec{r}_A - \vec{r}_B = (X_A - X_B,\; Y_A - Y_B) \\
\text{Moment arm of } \vec{W} \text{ about B}: \quad
& \vec{r}_{W/B} = \vec{r}_{\text{COM}} - \vec{r}_B = (X_{COM} - X_B,\; Y_{COM} - Y_B)
\end{align*}

Therefore,
\begin{align*}
    \sum \vec{F}_x &= -f_1 \cos\theta_1 + f_2 \cos\theta_2 
                     - N_A \sin\theta_1 - N_B \sin\theta_2 = 0 \\
    \sum \vec{F}_y &= f_1 \sin\theta_1 + f_2 \sin\theta_2 
                     - N_A \cos\theta_1 + N_B \cos\theta_2 - mg = 0 \\[1ex]
    \sum \vec{M}_A &= (X_B - X_A)(f_2 \sin\theta_2 + N_B \cos\theta_2)
                     - (Y_B - Y_A)(f_2 \cos\theta_2 - N_B \sin\theta_2)
                     - mg (X_{\text{COM}} - X_A) = 0 \\
    \sum \vec{M}_B &= (X_A - X_B)(f_1 \sin\theta_1 - N_A \cos\theta_1)
                     - (Y_A - Y_B)(-f_1 \cos\theta_1 - N_A \sin\theta_1)
                     - mg (X_{\text{COM}} - X_B) = 0
\end{align*}

solve,
\begin{align*}
    N_A &= \frac{g m (X_B - X_{\text{COM}}) \cos\theta_1}{X_A - X_B} \\[1ex]
    N_B &= \frac{g m (X_A - X_{\text{COM}}) \cos\theta_2}{X_A - X_B} \\[1ex]
    f_1 &= \frac{g m (X_{\text{COM}} - X_B) \sin\theta_1}{X_A - X_B} \\[1ex]
    f_2 &= \frac{g m (X_A - X_{\text{COM}}) \sin\theta_2}{X_A - X_B}
\end{align*}
    
By friction function \(\left| f \right| \leq \mu N\), we can solve this equation and find 

\begin{align*}
    \left| f_1 \right| &= \left| \frac{g m (X_{\text{COM}} - X_B) \sin\theta_1}{X_A - X_B} \right| 
    \leq \mu \cdot \frac{g m (X_B - X_{\text{COM}}) \cos\theta_1}{X_A - X_B} = \mu N_A \\[1.5ex]
    \left| f_2 \right| &= \left| \frac{g m (X_A - X_{\text{COM}}) \sin\theta_2}{X_A - X_B} \right| 
    \leq \mu \cdot \frac{g m (X_A - X_{\text{COM}}) \cos\theta_2}{X_A - X_B} = \mu N_B
\end{align*}

\begin{note}
    The above expression is derived in case where the \(\theta_1\) and \(\theta_2\) are both acute angles from graphic
    definition, but it is clear that in other cases, similar genral expression can also be formulated.
\end{note}
    
\subsection*{Cylinder Terrain}

\begin{diagram}
    Generailized expression on Cylinder Terrain
\end{diagram}
\vspace{1ex} % small vertical space
\begin{center}
    \includegraphics[width=0.8\textwidth]{figs/Generailized expression on Cylinder Terrain.jpg} % replace with your image
\end{center}

With the general expression, we can directly put the same graph within in a cylinder terrian, where
\(\theta_1\) and \(\theta_2\) are esseintially the tangent line with the cylinder. 

\begin{diagram}
    Impossible case under Assumption \ref{ass:leg-ground-contact}
\end{diagram}
\vspace{1ex} % small vertical space
\begin{center}
    \includegraphics[width=0.8\textwidth]{figs/Impossible case under Assumption.jpg} % replace with your image
\end{center}

However, here, it is impossible that right leg is still contacting the ground due to \(\beta\). In this case, the generalized 
geometric is not applied completely, which requires furthur discuss by changing the assumption \ref{ass:leg-ground-contact}. 

However, this case can also be determined geometrically. Now let's firstly simplify the problem
that all cylinder shape on this terrain has same radius. 

\subsubsection*{Cylinder Terrain when radius are identical}

I made a simple demo for robot geometric shape can be found in this \href{https://www.geogebra.org/classic/vzgc97bq}{GeoGebra link}.
Here A represents the contact point of left leg on the left circle and AB represents of \(L_{Spine}\). The
moving P point represents the right leg extension and AP represents the \(L_{Arm}\).For both folowing cases, 
we form equations as follows in coordinates:

\begin{note}
    In this terrain, what we actually want to consider is given the shape of the cylinder
    (i.e radius and gap), how can we find the \(\theta_1\) and \(\theta_2\).
\end{note}

\begin{diagram}
    When Point P contacts the terrain
\end{diagram}
\vspace{1ex} % small vertical space
\begin{center}
    \includegraphics[width=0.5\textwidth]{figs/Cylinder-Case1.jpg} % replace with your image
\end{center}

\begin{diagram}
    When Segment tangents the terrain
\end{diagram}
\vspace{1ex} % small vertical space
\begin{center}
    \includegraphics[width=0.5\textwidth]{figs/Cylinder-Case2.jpg} % replace with your image
\end{center}

\noindent\textbf{Obstacle and Terrain Representation}
\begin{align*}
    &\text{Obstacle } c_1&& (x - c_1)^2 + y^2 = r^2 \\\\
    &\text{Obstacle } c_2&& (x - c_2)^2 + y^2 = r^2
\end{align*}

% \noindent\textbf{Flat Terrain Between Obstacles:}
% \begin{equation*}
% \text{TerrainHeight}(x) =
% \begin{cases}
%     h_{\text{obs}}, & x < c_1 - r \\\\
%     h_{\text{gap}}, & c_1 + r \leq x \leq c_2 - r \\\\
%     h_{\text{obs}}, & x > c_2 + r \\\\
%     \text{undefined (wall)}, & \text{otherwise}
% \end{cases}
% \end{equation*}

\vspace{1em}
\noindent\textbf{Control Parameters}
\begin{align*}
    \theta &\in [0, \pi] 
    && \text{\small (defines point $A$ on the upper half of the circle centered at $c_1$)} \\ 
    \varphi &\in [0, 2\pi] 
    && \text{\small (controls the direction of the robot spine extended from point $A$)} \\ 
    s &\in [-L_{\text{leg}}, 0]
    && \text{\small (represents the extension length of the right leg from point $B$)}
\end{align*}

\vspace{1em}
\noindent\textbf{Point Definitions}
\begin{align*}
    A &= (x_0, y_0) = \left(c_1 + r \cos \theta,\ r \sin \theta\right) \\
    B &= (x_1, y_1) = \left(x_0 + L_{\text{spine}} \cos \varphi,\ y_0 + L_{\text{spine}} \sin \varphi\right)
\end{align*}
\vspace{1em}
\noindent\textbf{Body Reachability Circle}
\begin{align*}
    c_A: \quad (x - x_0)^2 + (y - y_0)^2 = L_{Spine}^2
\end{align*}

\vspace{1em}
\noindent\textbf{Direction Vector and Point P}
\begin{align*}
    \vec{t} &= (t_x, t_y) = (-\sin \varphi,\ \cos \varphi) \\
    P &= (x_P, y_P) = (x_1 + s t_x,\ y_1 + s t_y)
\end{align*}

% \vspace{1em}
% \noindent\textbf{Distances}
% \begin{align*}
%     L_{\text{arm}} &= \| \vec{AP} \| = \sqrt{(x_P - x_0)^2 + (y_P - y_0)^2} \\
%     L_{\text{spine}} &= \| \vec{AB} \| = \sqrt{(x_1 - x_0)^2 + (y_1 - y_0)^2}
% \end{align*}

\vspace{1em}
\noindent\textbf{Collision Condition}
% \begin{align*}
%     \text{InsideObstacle2}(P) &= (x_P - c_2)^2 + y_P^2 < r^2 \tag{\text{\small Point $P$ must remain outside Obstacle 2.}}
% \end{align*}
Generally speaking, segment \(\overline{BP}\)  must intersect the boundary of Obstacle 2 exactly once:
\begin{align*}
    \left| \overline{BP} \cap \partial c_2 \right| &= 1 \\
    \overline{BP} \cap c_2^\circ &= \emptyset
\end{align*}

% \noindent\textbf{Collision Condition (Point $(x, y)$ inside obstacle):}
% \begin{align*}
%     \text{InsideObstacle} &= \left[(x - c_1)^2 + y^2 < r^2\right] \lor \left[(x - c_2)^2 + y^2 < r^2\right]
% \end{align*}

\subsubsection*{Case1}
\indent \indent In this case, it is very similar to what we did in the previous sections that we would consider 
pitch angle \(\beta\) in consideration. With that, we can determine triangle with knowning that A and P are 
on \(c_1\) and \(c_2\) and their angle.

\begin{diagram}
    Determine the geometric shape
\end{diagram}
\vspace{1ex} % small vertical space
\begin{center}
    \includegraphics[width=0.5\textwidth]{figs/Cylinder-Case1-Supplementary.jpg} % replace with your image
\end{center}

\begin{itemize}
    \item Two circles $c_1$ and $c_2$ with centers $C_1 = (x_1, y_1)$ and $C_2 = (x_2, y_2)$ respectively, both of radius $r$.
    \item Unknown points $A \in \partial c_1$, $P \in \partial c_2$.
    \item Length $L = \|A - P\|$ is known.
    \item Direction angle of $\vec{AP}$ is known: $\psi \in [0, 2\pi]$ from pitch angle \(\beta\).
\end{itemize}

Then the direction vector is:
\[
\vec{d} = \vec{AP} = L(\cos \psi, \sin \psi)
\]

We parameterize:
\begin{align*}
A &= (x_A, y_A) \\
P &= A + \vec{d} = (x_A + L \cos \psi,\ y_A + L \sin \psi)
\end{align*}

Apply the circle constraints:
\begin{align*}
\|A - C_1\|^2 &= r^2 \tag{1} \\
\|P - C_2\|^2 &= r^2 \tag{2}
\end{align*}

Substituting into (2):
\begin{align*}
&\left( x_A + L \cos \psi - x_2 \right)^2 + \left( y_A + L \sin \psi - y_2 \right)^2 = r^2 \tag{2'}
\end{align*}

Now, equations (1) and (2') form a nonlinear system in $x_A, y_A$.

Once $A$ is solved, compute:
\begin{align*}
P &= A + L(\cos \psi, \sin \psi)
\end{align*}

Then, compute angle between $\vec{AP}$ and circle normals:
\begin{align*}
\theta_1 &= \arccos\left( \frac{(P - A) \cdot (A - C_1)}{L \cdot r} \right) \\
\theta_2 &= \arccos\left( \frac{(A - P) \cdot (P - C_2)}{L \cdot r} \right)
\end{align*}

These give the angles between the link $AP$ and the local radial directions at points $A$ and $P$.

\subsubsection*{Case2}

\indent \indent For case 2, we can express that tangent line for robot body reachability circle
at point B also must tanget with \(c_2\). Therefore we can formulate:
\begin{align*}
    &\text{Let } \vec{n} := B - A \\
    &\text{Define a line } \ell \text{ such that:} \\
    &\quad B \in \ell,\quad \vec{d}_\ell \cdot \vec{n} = 0 \quad \text{i.e., }\ell \text{ is tangent to } c_A \text{ at } B \\
    &\quad \exists\ P' \in \ell \cap \partial c_2,\quad \vec{d}_\ell \cdot (P' - C_2) = 0 \quad \text{i.e., } \ell \text{ is tangent to } c_2 \text{ at } P'\\
    &\quad \abs{BP'} \leq \abs{BP}
\end{align*}

\begin{note}
    For Case2, the pitch angle \(\beta\) does not matter and we can still find at most one solution.
\end{note}

Let $\vec{d}_\ell$ be the direction vector of $\ell$, defined by:
\begin{align*}
    \vec{d}_\ell &= (-n_y,\ n_x) \quad \text{(perpendicular to } \vec{n} = B - A\text{)}
\end{align*}

Then, the parametric equation of $\ell$ is:
\begin{align*}
    \ell(\lambda) &= B + \lambda \vec{d}_\ell
\end{align*}

To ensure tangency with $c_2$, we require:
\begin{align*}
    \|\ell(\lambda) - C_2\|^2 &= r^2
\end{align*}
which leads to a quadratic in $\lambda$:
\begin{align*}
    \|B + \lambda \vec{d}_\ell - C_2\|^2 &= r^2
\end{align*}

Solving this yields candidate point(s) $P' = B + \lambda^* \vec{d}_\ell$.
Select the point that satisfies:
\begin{align*}
    \|BP'\| &\leq \|BP\|
\end{align*}

Finally, the center $A$ of $c_A$ is obtained by inverting $\vec{n}$:
\begin{align*}
    \vec{n}_{\text{unit}} &= \frac{\vec{n}}{\|\vec{n}\|} \\
    A &= B - R \cdot \vec{n}_{\text{unit}}
\end{align*}

This determines $A$ and $P'$ geometrically under the tangency constraints.


\end{document}
